memabs/MemAbs.v
@@ -1,0 +1,221 @@
+Require Import Relations RelationClasses.
+Require Import List.
+Require Import compcert.common.LanguageInterface.
+Require Import compcert.common.Events.
+Require Import compcert.common.Globalenvs.
+Require Import models.Coherence.
+Require Import examples.CompCertSem.
+Require Import examples.Bigstep.
+Require Import compcert.cfrontend.Clight.
+Require Import compcert.common.Memory. (* mem *)
+Require Import compcert.common.AST.    (* Gvar *)
+Require Import compcert.cfrontend.Ctypes. (* type *)
+Require Import compcert.common.Values.    (* block *)
+Require Import compcert.lib.Integers.     (* ptrofs *)
+Require Import compcert.lib.Coqlib.       (* Z *)
+Require Import compcert.lib.Maps.         (* PTree.get *)
+Require Import compcert.common.Errors.    (* res *)
+Require Import compcert.common.Memory.    (* unchanged_on *)
+Require Import compcert.cfrontend.Cop.    (* val_casted_list *)
+Require Import compcert.common.Smallstep.
+
+(* Define a language interface with memory abstracted out *)
+Record d_query :=
+  dq {
+      dq_vf: val;
+      dq_sg: signature;
+      dq_args: list val;
+    }.
+Record d_reply :=
+  dr {
+      dr_retval: val;
+    }.
+Canonical Structure li_d :=
+  {|
+  query := d_query;
+  reply := d_reply;
+  entry := dq_vf;
+  |}.
+Inductive q_rel: query li_d -> query li_c -> mem -> Prop:=
+| q_rel_intro:
+    forall vf sg args m,
+      q_rel ({|dq_vf:=vf;dq_sg:=sg;dq_args:=args|})
+            ({|cq_vf:=vf;cq_sg:=sg;cq_args:=args;cq_mem:=m|}) m.
+Inductive r_rel: reply li_d -> reply li_c -> mem -> Prop:=
+  r_rel_intro:
+    forall ret m,
+      r_rel ({|dr_retval:=ret|})
+            ({|cr_retval:=ret;cr_mem:=m|}) m.
+Inductive qr_rel_list: list (query li_d * reply li_d) -> list (query li_c * reply li_c) -> Prop:=
+| qr_rel_nil: qr_rel_list nil nil
+| qr_rel_cons:
+    forall dq dr cq cr ds cs m m',
+      q_rel dq cq m ->
+      r_rel dr cr m' ->
+      qr_rel_list ds cs ->
+      qr_rel_list ((dq, dr)::ds) ((cq, cr)::cs).
+Inductive li_rel: (query li_d * reply li_d) -> (query li_c * reply li_c) -> Prop:=
+| rel_intro:
+    forall vf sg args ret m,
+      li_rel ({|dq_vf:=vf;dq_sg:=sg;dq_args:=args|}, {|dr_retval:=ret|})
+             ({|cq_vf:=vf;cq_sg:=sg;cq_args:=args;cq_mem:=m|}, {|cr_retval:=ret;cr_mem:=m|}).
+Local Obligation Tactic := idtac.
+Program Definition li_dc: li_d --o li_c :=
+  {|
+  has '(d, c) := li_rel d c
+  |}.
+Next Obligation.
+  intros [[dq1 dr1] [cq1 cr1]] [[dq2 dr2] [cq2 cr2]]. simpl.
+  intros rel1 rel2. intuition.
+  - destruct cq1. destruct cq2. inversion H. clear H. subst.
+    inversion rel1. subst. inversion rel2. subst.
+    f_equal. exploit H1. auto. congruence.
+  - injection H. destruct cr1. destruct cr2. destruct cq1. destruct cq2.
+    inversion rel1. inversion rel2. subst. intros.
+    f_equal. congruence. congruence.
+Defined.
+
+Section TRACE_STATE.
+  (* Since σ is not guaranteed to be a regular function, there is no way to "guess" the underlying 
+     behavior w that corresponds to (qx, rx) *)
+  Program Definition next {liA liB: language_interface} (σ : !liA --o !liB) w qx rx : !liA --o !liB :=
+    {|
+    has '(s, t) := has σ (w ++ s, (qx, rx)::t);
+    |}.
+  Next Obligation.
+    intros liA liB sig w q r [s1 t1] [s2 t2] H1 H2 Ht.
+    pose proof (has_coh _ _ _ _ H1 H2). cbn in H. clear H1 H2.
+    edestruct H as [Hr Hl].
+    apply (@app_coh liA). apply Ht.
+    split. inversion Hr. subst. apply H5. auto.
+    intro. exploit Hl. f_equal. auto. apply app_inv_head.
+  Qed.
+End TRACE_STATE.
+
+Module Sem1.
+  Section ABS_SEMANTICS.
+    Context {liA liB: language_interface} (Σ: !liA --o !liA) (C: Smallstep.semantics liB liB).
+    Variable li_rel: (query liA * reply liA) -> (query liB * reply liB) -> Prop.
+    Variable se: Genv.symtbl.
+
+    Variant state : Type := st (s: Smallstep.state C) (σ: !liA --o !liA).
+    
+    Inductive step: state -> trace -> state -> Prop :=
+    | step_internal: forall s s' t σ,
+        Step (C se) s t s' ->
+        step (st s σ) t (st s' σ)
+    | step_external: forall s s' qa ra qb rb σ w t,
+        Smallstep.at_external (C se) s qb ->
+        Smallstep.after_external (C se) s rb s' ->
+        has (next σ w qa ra) t ->
+        li_rel (qa, ra) (qb, rb) ->
+        step (st s σ) E0 (st s' (next σ w qa ra)).
+
+    Inductive initial_state: query liB -> state -> Prop :=
+    | initial_state_intro: forall q s,
+        Smallstep.initial_state (C se) q s ->
+        initial_state q (st s Σ).
+    (* We require Σ to account for all external calls of C *)
+    Inductive at_external: state -> query li_null -> Prop := .
+    Inductive after_external: state -> reply li_null -> state -> Prop := .
+    
+    Inductive final_state: state -> reply liB -> Prop :=
+    | final_state_intro: forall s r σ,
+        Smallstep.final_state (C se) s r ->
+        final_state (st s σ) r.
+
+    Definition lts : lts li_null liB state :=
+      {|
+      Smallstep.step _ := step;
+      Smallstep.valid_query := Smallstep.valid_query (C se);
+      Smallstep.initial_state := initial_state;
+      Smallstep.at_external := at_external;
+      Smallstep.after_external := after_external;
+      Smallstep.final_state := final_state;
+      Smallstep.globalenv := Smallstep.globalenv (C se);
+      |}.
+  End ABS_SEMANTICS.
+  Definition semantics_spec {liA liB: language_interface} skel li_rel (Σ: !liA --o !liA) (C: Smallstep.semantics liB liB) :=
+    {|
+    Smallstep.skel := skel;
+    Smallstep.activate se := lts Σ C li_rel se;
+    |}.
+  Definition c_semantics_spec (Σ: !li_d --o !li_d) (p: Clight.program): Smallstep.semantics li_null li_c :=
+    semantics_spec (AST.erase_program p) li_rel Σ (semantics1 p).
+End Sem1.
+
+Module Sem2.
+  Section IMPL_SEMANTICS.
+    Context {liA: language_interface} (σ: !liA --o liA) (C: Smallstep.semantics liA liA).
+    Variable se: Genv.symtbl.
+
+    Notation state := (Smallstep.state C).
+    
+    Inductive step: state -> trace -> state -> Prop :=
+    | step_internal: forall s s' t,
+        Step (C se) s t s' ->
+        step s t s'
+    | step_external: forall s s' q r t,
+        Smallstep.at_external (C se) s q ->
+        Smallstep.after_external (C se) s r s' ->
+        has σ (t, (q, r)) ->
+        step s E0 s'.
+    Inductive initial_state: query liA -> state -> Prop :=
+    | initial_state_intro: forall q s,
+        Smallstep.initial_state (C se) q s ->
+        initial_state q s.
+    Inductive at_external: state -> query li_null -> Prop := .
+    Inductive after_external: state -> reply li_null -> state -> Prop := .
+    
+    Inductive final_state: state -> reply liA -> Prop :=
+    | final_state_intro: forall s r,
+        Smallstep.final_state (C se) s r ->
+        final_state s r.
+
+    Definition lts : lts li_null liA state :=
+      {|
+      Smallstep.step _ := step;
+      Smallstep.valid_query := Smallstep.valid_query (C se);
+      Smallstep.initial_state := initial_state;
+      Smallstep.at_external := at_external;
+      Smallstep.after_external := after_external;
+      Smallstep.final_state := final_state;
+      Smallstep.globalenv := Smallstep.globalenv (C se);
+      |}.
+  End IMPL_SEMANTICS.
+  Definition semantics_impl {liA: language_interface} skel (σ: !liA --o liA) (C: Smallstep.semantics liA liA) :=
+    {|
+    Smallstep.skel := skel;
+    Smallstep.activate se := lts σ C se;
+    |}.
+  Definition c_semantics_impl (σ: !li_c --o li_c) (p: Clight.program): Smallstep.semantics li_null li_c :=
+    semantics_impl (AST.erase_program p) σ (semantics1 p).
+End Sem2.
+
+Section ABS_CKLR.
+  Variable ge: genv.
+  
+  Inductive module_var: ident -> type -> block -> ptrofs -> Prop :=
+  | module_var_intro id b (v : globvar type) (ty : type):
+      Genv.find_symbol ge id = Some b ->
+      Genv.find_def ge b = Some (Gvar v) ->
+      ty = gvar_info v ->
+      module_var id ty b Ptrofs.zero.
+
+  Inductive abs_world :=
+    absw (vals: PTree.t val).
+
+  Inductive value_match (ty: type) (m: mem) (b: block) (ofs: ptrofs): option val -> Prop :=
+  | value_match_some v:
+      deref_loc ty m b ofs v ->
+      value_match ty m b ofs (Some v).
+  Inductive abs_match_mem: abs_world -> relation mem :=
+    abs_match_mem_intro m1 m2 vs:
+      Mem.extends m1 m2 ->
+      (forall id ty b ofs,
+          module_var id ty b ofs ->
+          (forall k p, ~Mem.perm m1 b (Ptrofs.unsigned ofs) k p) /\
+          value_match ty m2 b ofs (vs ! id)) ->
+      abs_match_mem (absw vs) m1 m2.
+  
+End ABS_CKLR.
